

Assignment 3 D

Date _____

Page No. _____

$$I = \begin{bmatrix} 1 & 2 & 0 & 1 \\ 3 & 1 & 2 & 2 \\ 0 & 1 & 3 & 1 \\ 2 & 2 & 2 & 0 \end{bmatrix}$$

$$K_1 = \begin{bmatrix} 1 & 0 & -1 \\ 1 & 0 & -1 \\ 1 & 0 & -1 \end{bmatrix} \quad K_2 = \begin{bmatrix} 1 & 1 & 0 \\ 0 & 1 & 0 \\ 0 & 1 & 0 \end{bmatrix}$$

$$\begin{aligned} H_{out} &= (H - K + 2P/s) + \frac{1}{s} \\ &= 14 - 3 + 0/1 + 1 \\ &= 2 \quad H_{out} = 2 \end{aligned}$$

from K_1 ,

$$\begin{bmatrix} 1 & 2 & 0 \\ 3 & 1 & 2 \\ 0 & 1 & 3 \end{bmatrix} \times \begin{bmatrix} 1 & 0 & -1 \\ 1 & 0 & -1 \\ 1 & 0 & -1 \end{bmatrix}$$

$$= 1 \cdot 1 + 2 \cdot 0 + 0 \cdot 1 + 3 \cdot 1 + 1 \cdot 0 + 2 \cdot 1 + 0 \cdot 1 + 1 \cdot 0 + 3 \cdot 1$$

$$= 1 + 3 - 2 - 3$$

$$= -1$$

$$\begin{bmatrix} 2 & 0 & 1 \\ 1 & 2 & 2 \\ 1 & 3 & 1 \end{bmatrix} \times \begin{bmatrix} 1 & 0 & -1 \\ 1 & 0 & -1 \\ 1 & 0 & -1 \end{bmatrix}$$

$$= 2 \cdot 1 + 0 \cdot 0 + 1 \cdot (-1) + 1 \cdot 1 + 2 \cdot 0 + 2 \cdot 1 + 1 \cdot 1 + 3 \cdot 0 + 1 \cdot (-1)$$

$$= 2 - 1 + 1 - 2 + 1 - 1$$

$$= 0$$

$$\begin{bmatrix} 3 & 1 & 2 \\ 0 & 1 & 3 \\ 2 & 2 & 2 \end{bmatrix} \times \begin{bmatrix} 1 & 0 & -1 \\ 1 & 0 & -1 \\ 1 & 0 & -1 \end{bmatrix}$$

$$= 3 \cdot 1 + 1 \cdot 0 + 2 \cdot (-1) + 0 \cdot 1 + 1 \cdot 0 + 3 \cdot (-1) + 2 \cdot 1 + 2 \cdot 0 + 2 \cdot (-1)$$

$$= 3 - 2 - 3 + 2 - 2$$

$$= -2$$

$$\begin{bmatrix} 1 & 2 & 2 \\ 1 & 3 & 1 \\ 2 & 2 & 0 \end{bmatrix} \times \begin{bmatrix} 1 & 0 & -1 \\ 1 & 0 & -1 \\ 1 & 0 & -1 \end{bmatrix}$$

$$= 1 \cdot 1 + 2 \cdot 0 + 2 \cdot (-1) + 1 \cdot 1 + 3 \cdot 0 + 1 \cdot (-1) + 2 \cdot 1 + 2 \cdot 0 + 0 \cdot (-1)$$

$$= 1 - 2 + 1 - 1 + 2$$

$$= 1$$

Output from kernel 1 is $\begin{bmatrix} -1 & 0 \\ -2 & 1 \end{bmatrix}$

Using K_2 .

$$\begin{bmatrix} 1 & 2 & 0 \\ 3 & 1 & 2 \\ 0 & 1 & 3 \end{bmatrix} \times \begin{bmatrix} 0 & 1 & 0 \\ 0 & 1 & 0 \\ 0 & 1 & 0 \end{bmatrix}$$

$$= 1 \cdot 0 + 2 \cdot 1 + 0 \cdot 0 + 3 \cdot 0 + 1 \cdot 1 + 2 \cdot 0 + 0 \cdot 0 + 1 \cdot 1 + 3 \cdot 0$$

$$= 2 + 1 + 1$$

$$= 4$$

$$\begin{bmatrix} 2 & 0 & 1 \\ 1 & 2 & 2 \\ 1 & 3 & 1 \end{bmatrix} \times \begin{bmatrix} 0 & 1 & 0 \\ 0 & 1 & 0 \\ 0 & 1 & 0 \end{bmatrix}$$

$$= 2 \cdot 0 + 0 \cdot 1 + 1 \cdot 0 + 1 \cdot 0 + 2 \cdot 1 + 2 \cdot 0 + 1 \cdot 0 + 3 \cdot 1 + 1 \cdot 0$$

$$= 2 + 3$$

$$= 5$$

$$\begin{bmatrix} 3 & 1 & 2 \\ 0 & 1 & 3 \\ 2 & 2 & 2 \end{bmatrix} \times \begin{bmatrix} 0 & 1 & 0 \\ 0 & 1 & 0 \\ 0 & 1 & 0 \end{bmatrix}$$

$$= 3 \cdot 0 + 1 \cdot 1 + 2 \cdot 0 + 0 \cdot 0 + 1 \cdot 1 + 3 \cdot 0 + 2 \cdot 0 + 2 \cdot 1 + 2 \cdot 0$$

$$= 1 + 1 + 2$$

$$= 4$$

$$\begin{bmatrix} 1 & 2 & 2 \\ 1 & 3 & 1 \\ 2 & 2 & 0 \end{bmatrix} \times \begin{bmatrix} 0 & 1 & 0 \\ 0 & 1 & 0 \\ 0 & 1 & 0 \end{bmatrix}$$

$$= 1 \cdot 0 + 2 \cdot 1 + 2 \cdot 0 + 1 \cdot 0 + 3 \cdot 1 + 1 \cdot 0 + 2 \cdot 0 + 2 \cdot 1 + 0 \cdot 0$$

$$= 2 + 3 + 2$$

$$= 7$$

Output from kernel 2 is $\begin{bmatrix} 4 & 5 \\ 4 & 7 \end{bmatrix}$